TransitionSystems WIP

Invariant.v
@@ -1,35 +1,41 @@
 Require Import Relations.
 
+Set Implicit Arguments.
 
-Definition invariantFor {state} (initial : state -> Prop) (step : state -> state -> Prop) (invariant : state -> Prop) :=
-  forall s, initial s
-            -> forall s', step^* s s'
+
+Record trsys state := {
+  Initial : state -> Prop;
+  Step : state -> state -> Prop
+}.
+
+Definition invariantFor {state} (sys : trsys state) (invariant : state -> Prop) :=
+  forall s, sys.(Initial) s
+            -> forall s', sys.(Step)^* s s'
                           -> invariant s'.
 
-Theorem use_invariant : forall {state} (initial : state -> Prop)
-  (step : state -> state -> Prop) (invariant : state -> Prop) s s',
-  step^* s s'
-  -> initial s
-  -> invariantFor initial step invariant
+Theorem use_invariant : forall {state} (sys : trsys state) (invariant : state -> Prop) s s',
+  sys.(Step)^* s s'
+  -> sys.(Initial) s
+  -> invariantFor sys invariant
   -> invariant s'.
 Proof.
   firstorder.
 Qed.
 
-Theorem invariantFor_monotone : forall {state} (initial : state -> Prop)
-  (step : state -> state -> Prop) (invariant1 invariant2 : state -> Prop),
+Theorem invariantFor_monotone : forall {state} (sys : trsys state)
+  (invariant1 invariant2 : state -> Prop),
   (forall s, invariant1 s -> invariant2 s)
-  -> invariantFor initial step invariant1
-  -> invariantFor initial step invariant2.
+  -> invariantFor sys invariant1
+  -> invariantFor sys invariant2.
 Proof.
   unfold invariantFor; intuition eauto.
 Qed.
 
-Theorem invariant_induction : forall {state} (initial : state -> Prop)
-  (step : state -> state -> Prop) (invariant : state -> Prop),
-  (forall s, initial s -> invariant s)
-  -> (forall s, invariant s -> forall s', step s s' -> invariant s')
-  -> invariantFor initial step invariant.
+Theorem invariant_induction : forall {state} (sys : trsys state)
+  (invariant : state -> Prop),
+  (forall s, sys.(Initial) s -> invariant s)
+  -> (forall s, invariant s -> forall s', sys.(Step) s s' -> invariant s')
+  -> invariantFor sys invariant.
 Proof.
   unfold invariantFor; intros.
   assert (invariant s) by eauto.
